{
 "cells": [
  {
   "cell_type": "markdown",
   "id": "5bb60ca3",
   "metadata": {},
   "source": [
    "### 1. Find the value of T(2) for the recurrence relation T(n) = 3T(n-1) + 12n, given that T(0)=5."
   ]
  },
  {
   "cell_type": "code",
   "execution_count": 1,
   "id": "12a78e12",
   "metadata": {},
   "outputs": [
    {
     "name": "stdout",
     "output_type": "stream",
     "text": [
      "T(2) = 105\n"
     ]
    }
   ],
   "source": [
    "def recurrence_relation(n):\n",
    "    if n == 0:\n",
    "        return 5\n",
    "    else:\n",
    "        return 3 * recurrence_relation(n - 1) + 12 * n\n",
    "\n",
    "result = recurrence_relation(2)\n",
    "\n",
    "print(\"T(2) =\", result)"
   ]
  },
  {
   "cell_type": "markdown",
   "id": "b2580abd",
   "metadata": {},
   "source": [
    "### 2. Given a recurrence relation, solve it using the substitution method:\n",
    "#### a. T(n) = T(n-1) + c\n",
    "#### b. T(n) = 2T(n/2) + n\n",
    "#### c. T(n) = 2T(n/2) + c\n",
    "#### d. T(n) = T(n/2) + c"
   ]
  },
  {
   "cell_type": "markdown",
   "id": "b7ecac14",
   "metadata": {},
   "source": [
    "Solution to the given recurrence relations using the substitution method:\n",
    "\n",
    "### a. \\( T(n) = T(n-1) + c \\)\n",
    "\n",
    "**Substitution:**\n",
    "\n",
    "- Start by expanding the recurrence relation step by step:\n",
    "\n",
    "\\[\n",
    "T(n) = T(n-1) + c\n",
    "\\]\n",
    "\n",
    "\\[\n",
    "T(n-1) = T(n-2) + c\n",
    "\\]\n",
    "\n",
    "\\[\n",
    "T(n-2) = T(n-3) + c\n",
    "\\]\n",
    "\n",
    "- Continuing this pattern until the base case \\( T(1) = T(0) + c \\), we get:\n",
    "\n",
    "\\[\n",
    "T(n) = T(n-2) + 2c = T(n-3) + 3c = \\dots = T(1) + (n-1)c\n",
    "\\]\n",
    "\n",
    "\\[\n",
    "T(n) = T(1) + (n-1)c\n",
    "\\]\n",
    "\n",
    "Assuming \\( T(1) = T(0) = c \\):\n",
    "\n",
    "\\[\n",
    "T(n) = c + (n-1)c = nc\n",
    "\\]\n",
    "\n",
    "**Solution:**\n",
    "\n",
    "\\[\n",
    "T(n) = O(n)\n",
    "\\]\n",
    "\n",
    "### b. \\( T(n) = 2T(n/2) + n \\)\n",
    "\n",
    "**Substitution:**\n",
    "\n",
    "- Let's assume \\( T(n) = n \\log_2 n \\) and substitute it into the recurrence:\n",
    "\n",
    "\\[\n",
    "T(n) = 2 \\left(\\frac{n}{2} \\log_2 \\frac{n}{2} \\right) + n\n",
    "\\]\n",
    "\n",
    "- Simplify the right-hand side:\n",
    "\n",
    "\\[\n",
    "T(n) = 2 \\left(\\frac{n}{2} (\\log_2 n - 1) \\right) + n = n \\log_2 n - n + n = n \\log_2 n\n",
    "\\]\n",
    "\n",
    "**Solution:**\n",
    "\n",
    "\\[\n",
    "T(n) = O(n \\log_2 n)\n",
    "\\]\n",
    "\n",
    "### c. \\( T(n) = 2T(n/2) + c \\)\n",
    "\n",
    "**Substitution:**\n",
    "\n",
    "- Start by expanding the recurrence:\n",
    "\n",
    "\\[\n",
    "T(n) = 2T(n/2) + c\n",
    "\\]\n",
    "\n",
    "\\[\n",
    "T(n/2) = 2T(n/4) + c\n",
    "\\]\n",
    "\n",
    "\\[\n",
    "T(n/4) = 2T(n/8) + c\n",
    "\\]\n",
    "\n",
    "- Expanding until we reach the base case:\n",
    "\n",
    "\\[\n",
    "T(n) = 2\\left(2T(n/4) + c\\right) + c = 4T(n/4) + 2c + c = 4\\left(2T(n/8) + c\\right) + 2c + c\n",
    "\\]\n",
    "\n",
    "- Generalizing this pattern, after \\( k \\) steps:\n",
    "\n",
    "\\[\n",
    "T(n) = 2^k T(n/2^k) + kc\n",
    "\\]\n",
    "\n",
    "- If we set \\( k = \\log_2 n \\), then \\( T(n/2^k) = T(1) \\), so:\n",
    "\n",
    "\\[\n",
    "T(n) = 2^{\\log_2 n} T(1) + \\log_2 n \\cdot c = nT(1) + c \\log_2 n\n",
    "\\]\n",
    "\n",
    "Assuming \\( T(1) = c \\):\n",
    "\n",
    "\\[\n",
    "T(n) = cn + c \\log_2 n\n",
    "\\]\n",
    "\n",
    "**Solution:**\n",
    "\n",
    "\\[\n",
    "T(n) = O(n)\n",
    "\\]\n",
    "\n",
    "### d. \\( T(n) = T(n/2) + c \\)\n",
    "\n",
    "**Substitution:**\n",
    "\n",
    "- Start by expanding the recurrence:\n",
    "\n",
    "\\[\n",
    "T(n) = T(n/2) + c\n",
    "\\]\n",
    "\n",
    "\\[\n",
    "T(n/2) = T(n/4) + c\n",
    "\\]\n",
    "\n",
    "\\[\n",
    "T(n/4) = T(n/8) + c\n",
    "\\]\n",
    "\n",
    "- Expanding until we reach the base case \\( T(1) = c \\):\n",
    "\n",
    "\\[\n",
    "T(n) = T(1) + c \\log_2 n\n",
    "\\]\n",
    "\n",
    "Since \\( T(1) = c \\):\n",
    "\n",
    "\\[\n",
    "T(n) = c \\log_2 n + c\n",
    "\\]\n",
    "\n",
    "**Solution:**\n",
    "\n",
    "\\[\n",
    "T(n) = O(\\log_2 n)\n",
    "\\]"
   ]
  },
  {
   "cell_type": "markdown",
   "id": "b9c051e5",
   "metadata": {},
   "source": [
    "### 3. Given a recurrence relation, solve it using the recursive tree approach:\n",
    "#### a. T(n) = 2T(n-1) +1\n",
    "#### b. T(n) = 2T(n/2) + n"
   ]
  },
  {
   "cell_type": "markdown",
   "id": "cb30c570",
   "metadata": {},
   "source": [
    "Hereâ€™s how you can solve the given recurrence relations using the recursive tree approach:\n",
    "\n",
    "### 3. Given a recurrence relation, solve it using the recursive tree approach:\n",
    "\n",
    "#### a. \\( T(n) = 2T(n-1) + 1 \\)\n",
    "\n",
    "**Recursive Tree Approach:**\n",
    "\n",
    "1. **Expand the Recurrence:**\n",
    "   - Start by expanding the recurrence for a few levels to see the pattern.\n",
    "\n",
    "\\[\n",
    "T(n) = 2T(n-1) + 1\n",
    "\\]\n",
    "\n",
    "\\[\n",
    "T(n-1) = 2T(n-2) + 1\n",
    "\\]\n",
    "\n",
    "\\[\n",
    "T(n-2) = 2T(n-3) + 1\n",
    "\\]\n",
    "\n",
    "2. **Construct the Tree:**\n",
    "   - At each level, the function splits into two calls, and each call reduces the problem size by 1.\n",
    "\n",
    "\\[\n",
    "T(n) = 2\\left(2T(n-2) + 1\\right) + 1 = 4T(n-2) + 2 + 1\n",
    "\\]\n",
    "\n",
    "   - Continue expanding:\n",
    "\n",
    "\\[\n",
    "T(n) = 4\\left(2T(n-3) + 1\\right) + 2 + 1 = 8T(n-3) + 4 + 2 + 1\n",
    "\\]\n",
    "\n",
    "3. **Generalize the Pattern:**\n",
    "   - The tree depth is \\( n \\), and at the bottom level, there are \\( 2^k \\) leaves, each contributing \\( T(n-k) \\).\n",
    "\n",
    "   - The sum of contributions from all levels is:\n",
    "\n",
    "\\[\n",
    "T(n) = 2^0 + 2^1 + 2^2 + \\dots + 2^{n-1}\n",
    "\\]\n",
    "\n",
    "4. **Calculate the Sum:**\n",
    "   - The sum of a geometric series:\n",
    "\n",
    "\\[\n",
    "T(n) = 2^n - 1\n",
    "\\]\n",
    "\n",
    "**Solution:**\n",
    "\n",
    "\\[\n",
    "T(n) = O(2^n)\n",
    "\\]\n",
    "\n",
    "The recurrence relation can be represented as follows:\n",
    "\n",
    "          T(n)\n",
    "         /    \\\n",
    "      T(n-1)   T(n-1)\n",
    "       / \\      / \\\n",
    "   T(n-2) T(n-2) T(n-2) T(n-2)\n",
    "    / \\    / \\    / \\    / \\\n",
    "T(n-3) T(n-3) T(n-3) T(n-3) ...\n",
    "\n",
    "#### b. \\( T(n) = 2T(n/2) + n \\)\n",
    "\n",
    "**Recursive Tree Approach:**\n",
    "\n",
    "1. **Expand the Recurrence:**\n",
    "   - Start by expanding the recurrence for a few levels:\n",
    "\n",
    "\\[\n",
    "T(n) = 2T(n/2) + n\n",
    "\\]\n",
    "\n",
    "\\[\n",
    "T(n/2) = 2T(n/4) + \\frac{n}{2}\n",
    "\\]\n",
    "\n",
    "\\[\n",
    "T(n/4) = 2T(n/8) + \\frac{n}{4}\n",
    "\\]\n",
    "\n",
    "2. **Construct the Tree:**\n",
    "   - The problem size reduces by half at each level, and each level contributes a total cost proportional to the original problem size \\( n \\).\n",
    "\n",
    "3. **Generalize the Pattern:**\n",
    "   - The number of levels in the tree is \\( \\log_2 n \\).\n",
    "   - Each level contributes \\( n \\).\n",
    "\n",
    "\\[\n",
    "T(n) = n + n + n + \\dots + n\n",
    "\\]\n",
    "\n",
    "   - There are \\( \\log_2 n \\) levels.\n",
    "\n",
    "4. **Calculate the Sum:**\n",
    "\n",
    "\\[\n",
    "T(n) = n \\log_2 n\n",
    "\\]\n",
    "\n",
    "**Solution:**\n",
    "\n",
    "\\[\n",
    "T(n) = O(n \\log_2 n)\n",
    "\\]\n",
    "\n",
    "The recurrence relation can be represented as follows:\n",
    "\n",
    "                    T(n)\n",
    "                 /         \\\n",
    "            T(n/2)       T(n/2)\n",
    "           /     \\       /     \\\n",
    "      T(n/4)  T(n/4) T(n/4)  T(n/4)\n",
    "       .         .      .       .\n",
    "       .         .      .       .\n",
    "       .         .      .       ."
   ]
  },
  {
   "cell_type": "markdown",
   "id": "bcfcbd6d",
   "metadata": {},
   "source": []
  }
 ],
 "metadata": {
  "kernelspec": {
   "display_name": "Python 3 (ipykernel)",
   "language": "python",
   "name": "python3"
  },
  "language_info": {
   "codemirror_mode": {
    "name": "ipython",
    "version": 3
   },
   "file_extension": ".py",
   "mimetype": "text/x-python",
   "name": "python",
   "nbconvert_exporter": "python",
   "pygments_lexer": "ipython3",
   "version": "3.11.4"
  }
 },
 "nbformat": 4,
 "nbformat_minor": 5
}
